core/Semantics.v
@@ -17,11 +17,9 @@ Context {tc: TransformationConfiguration}.
 
 (** * Instantiate **)
 
-Definition matchRuleOnPattern (r: Rule) (sm : SourceModel) (sp: list SourceModelElement) : bool :=
-  match evalGuardExpr r sm sp with Some true => true | _ => false end.
 
 Definition matchPattern (tr: Transformation) (sm : SourceModel) (sp: list SourceModelElement) : list Rule :=
-  filter (fun (r:Rule) => matchRuleOnPattern r sm sp) tr.(rules).
+  filter (fun (r:Rule) => evalGuardExpr r sm sp) tr.(rules).
 
 Definition instantiateElementOnPattern (o: OutputPatternElement) (sm: SourceModel) (sp: list SourceModelElement) (iter: nat)
   : option TargetModelElement :=
